Algoritmos Aproximados/Envasado.dfy/EnvasadoKAproximado.dfy
@@ -3,6 +3,6 @@ include "../../Especificaciones/Envasado/Envasado.dfy"
 //Definition of what it means for a solution to be K-Aproximated in the Bin Packing Problem
 ghost predicate isKAproximatedBinPacking(A : multiset<nat>, E : nat, I:multiset<multiset<nat>>, k: nat)
 {
-       isEnvasado(A, E, I)
-    && forall I': multiset<multiset<nat>> | isEnvasado(A, E, I') :: |I| <= |I'| * k
+       isBinPacking(A, E, I)
+    && forall I': multiset<multiset<nat>> | isBinPacking(A, E, I') :: |I| <= |I'| * k
 }
